working on wp with traces

theories/program_logic/traces.v
@@ -1,5 +1,5 @@
 From aneris.prelude Require Export fixpoint classical.
-From aneris.program_logic Require Export weakestpre.
+From aneris.program_logic Require Export language.
 
 Set Default Proof Using "Type".
 
@@ -28,208 +28,169 @@ Section finite_trace_lib.
     | trace_extend _ a => a
     end.
 
+  Definition trace_starts_in (ft : finite_trace A) (a : A) : Prop :=
+    trace_first ft = a.
+
+  Definition trace_ends_in (ft : finite_trace A) (a : A) : Prop :=
+    trace_last ft = a.
+
+  Lemma trace_singleton_starts_in c : trace_starts_in (trace_singleton c) c.
+  Proof. done. Qed.
+
+  Lemma trace_singleton_starts_in_inv c c' :
+    trace_starts_in (trace_singleton c') c → c' = c.
+  Proof. by inversion 1. Qed.
+
+  Lemma trace_singleton_ends_in c : trace_ends_in (trace_singleton c) c.
+  Proof. done. Qed.
+
+  Lemma trace_singleton_ends_in_inv c c' :
+    trace_ends_in (trace_singleton c') c → c' = c.
+  Proof. by inversion 1. Qed.
+
+  Lemma trace_starts_in_inj ex c c' :
+   trace_starts_in ex c → trace_starts_in ex c' → c = c'.
+  Proof. rewrite /trace_starts_in; intros ->; done. Qed.
+
+  Lemma trace_ends_in_inj ex c c' :
+   trace_ends_in ex c → trace_ends_in ex c' → c = c'.
+  Proof. rewrite /trace_ends_in; intros ->; done. Qed.
+
+  Definition trace_contract (ft ft' : finite_trace A) : Prop :=
+    ∃ a, ft = trace_extend ft' a.
+
+  Lemma trace_contract_of_extend ft a ft' :
+    trace_contract (trace_extend ft a) ft' → ft' = ft.
+  Proof. intros (? & Heq); simplify_eq; done. Qed.
+
+  Lemma not_trace_contract_singleton a ft :
+    ¬ trace_contract (trace_singleton a) ft.
+  Proof. intros (?&?); destruct ft; simplify_eq/=. Qed.
+
+  Lemma trace_extend_starts_in ft a' a :
+    trace_starts_in ft a' → trace_starts_in (trace_extend ft a) a'.
+  Proof. induction ft; auto. Qed.
+
+  Lemma trace_extend_starts_in_inv ft a' a :
+    trace_starts_in (trace_extend ft a) a' → trace_starts_in ft a'.
+  Proof. induction ft; auto. Qed.
+
+  Lemma trace_extend_ends_in ex c : trace_ends_in (trace_extend ex c) c.
+  Proof. done. Qed.
+
+  Lemma trace_does_ends_in ft : ∃ a, trace_ends_in ft a.
+  Proof. destruct ft; rewrite /trace_ends_in; eauto. Qed.
+
 End finite_trace_lib.
 
 Definition execution_trace Λ := finite_trace (cfg Λ).
+
+Record AuxState Λ : Type := {
+  (** Auxiliary state tracked along the physical state. *)
+  aux_state : Type;
+
+  auxiliary_trace := finite_trace aux_state;
+
+  (** The relation between the state before and after every step. *)
+  valid_state_evolution :
+    finite_trace (cfg Λ) → finite_trace aux_state → cfg Λ → aux_state → Prop;
+
+  (** We can always take a valid step in the auxiliary state *)
+  pure_step_evolution_valid extr atr c1 δ1 :
+    trace_ends_in extr c1 →
+    trace_ends_in atr δ1 →
+    valid_state_evolution extr atr c1 δ1;
+}.
+
+Arguments aux_state {_}.
+Arguments auxiliary_trace {_}.
+Arguments valid_state_evolution {_ _}, {_} _.
+Arguments pure_step_evolution_valid {_}.
 
 Section execution_trace.
   Context {Λ : language}.
 
   Implicit Types c : cfg Λ.
 
-  Definition singleton_exec (c : cfg Λ) : execution_trace Λ :=
-    trace_singleton c.
-
-  Definition exec_starts_in (ex : execution_trace Λ) (c : cfg Λ) : Prop :=
-    trace_first ex = c.
-
-  Definition exec_ends_in (ex : execution_trace Λ) (c : cfg Λ) : Prop :=
-    trace_last ex = c.
-
-  Lemma singleton_exec_starts_in c : exec_starts_in (singleton_exec c) c.
-  Proof. done. Qed.
-
-  Lemma singleton_exec_starts_in_inv c c' :
-    exec_starts_in (singleton_exec c') c → c' = c.
-  Proof. by inversion 1. Qed.
-
-  Lemma singleton_exec_ends_in c : exec_ends_in (singleton_exec c) c.
-  Proof. done. Qed.
-
-  Lemma singleton_exec_ends_in_inv c c' :
-    exec_ends_in (singleton_exec c') c → c' = c.
-  Proof. by inversion 1. Qed.
-
-  Lemma exec_ends_in_inj ex c c' :
-    exec_ends_in ex c → exec_ends_in ex c' → c = c'.
-  Proof. rewrite /exec_ends_in; intros ->; congruence. Qed.
-
-  Definition exec_extend (ex : execution_trace Λ) (c : cfg Λ) :=
-    trace_extend ex c.
-
-  Definition exec_contract (ex ex' : execution_trace Λ) : Prop :=
-    ∃ c, ex = exec_extend ex' c.
-
-  Lemma exec_contract_of_extend ex c ex' :
-    exec_contract (exec_extend ex c) ex' → ex' = ex.
-  Proof.
-    rewrite /exec_contract /exec_extend.
-    intros (? & Heq); simplify_eq.
-    repeat match goal with
-             Heq : _ |- _ => apply app_singleton_inv in Heq as [? ?]
-           end; simplify_eq; done.
-  Qed.
-
-  Lemma not_exec_contract_singleton c ex :
-    ¬ exec_contract (singleton_exec c) ex.
-  Proof. intros (?&?); destruct ex; simplify_eq/=. Qed.
-
   Inductive valid_exec : execution_trace Λ → Prop :=
-  | valid_exec_singleton c : valid_exec (singleton_exec c)
+  | valid_exec_singleton c : valid_exec (trace_singleton c)
   | valid_exec_step ex c c' :
-      exec_ends_in ex c →
+      trace_ends_in ex c →
       step c c' →
       valid_exec ex →
-      valid_exec (exec_extend ex c').
+      valid_exec (trace_extend ex c').
 
-  Lemma valid_singleton_exec c : valid_exec (singleton_exec c).
+  Lemma valid_singleton_exec c : valid_exec (trace_singleton c).
   Proof. constructor. Qed.
-
-  Lemma exec_extend_starts_in ex c' c :
-    exec_starts_in ex c' → exec_starts_in (exec_extend ex c) c'.
-  Proof. induction ex; auto. Qed.
-
-  Lemma exec_extend_starts_in_inv ex c' c :
-    exec_starts_in (exec_extend ex c) c' →
-    exec_starts_in ex c'.
-  Proof. induction ex; auto. Qed.
-
-  Lemma exec_extend_ends_in ex c : exec_ends_in (exec_extend ex c) c.
-  Proof. done. Qed.
-
-  Lemma valid_exec_ends_in ex : ∃ c, exec_ends_in ex c.
-  Proof. destruct ex; rewrite /exec_ends_in; eauto. Qed.
 
   Lemma extend_valid_exec ex c c':
     valid_exec ex →
-    exec_ends_in ex c →
+    trace_ends_in ex c →
     step c c' →
-    valid_exec (exec_extend ex c').
+    valid_exec (trace_extend ex c').
   Proof.
     intros He; revert c c'.
     induction ex; econstructor; eauto.
   Qed.
 
   Lemma valid_exec_exec_extend_inv ex c':
-    valid_exec (exec_extend ex c') →
+    valid_exec (trace_extend ex c') →
     valid_exec ex ∧
-    ∃ c, exec_ends_in ex c ∧ step c c'.
+    ∃ c, trace_ends_in ex c ∧ step c c'.
   Proof. inversion 1; eauto. Qed.
 
 End execution_trace.
 
-Definition auxiliary_trace {Λ} (AS : AuxState Λ) := finite_trace (aux_state AS).
-
-Section auxiliary_trace.
-  Context `{AS : AuxState Λ}.
-
-  Definition singleton_auxtr (δ : aux_state AS) : auxiliary_trace AS :=
-    trace_singleton δ.
-
-  Definition auxtr_starts_in
-             (atr : auxiliary_trace AS) (δ : aux_state AS) : Prop :=
-    trace_first atr = δ.
-
-  Definition auxtr_ends_in (atr : auxiliary_trace AS) (δ : aux_state AS)
-    : Prop := trace_last atr = δ.
-
-  Lemma singleton_auxtr_starts_in δ : auxtr_starts_in (singleton_auxtr δ) δ.
-  Proof. done. Qed.
-
-  Lemma singleton_auxtr_starts_in_inv δ δ' :
-    auxtr_starts_in (singleton_auxtr δ') δ → δ' = δ.
-  Proof. by inversion 1. Qed.
-
-  Lemma singleton_auxtr_ends_in δ : auxtr_ends_in (singleton_auxtr δ) δ.
-  Proof. done. Qed.
-
-  Lemma singleton_auxtr_ends_in_inv δ δ' :
-    auxtr_ends_in (singleton_auxtr δ') δ → δ' = δ.
-  Proof. by inversion 1. Qed.
-
-  Lemma auxtr_ends_in_inj atr δ δ' :
-    auxtr_ends_in atr δ → auxtr_ends_in atr δ' → δ = δ'.
-  Proof. rewrite /auxtr_ends_in; intros ->; congruence. Qed.
-
-  Definition auxtr_extend (atr : auxiliary_trace AS) (δ : aux_state AS) :=
-    trace_extend atr δ.
-
-  Definition auxtr_contract (atr atr' : auxiliary_trace AS) : Prop :=
-    ∃ δ, atr = auxtr_extend atr' δ.
-
-  Lemma auxtr_contract_of_extend atr δ atr' :
-    auxtr_contract (auxtr_extend atr δ) atr' → atr' = atr.
-  Proof. intros [? ?]; simplify_eq; done. Qed.
-
-  Lemma auxtr_extend_starts_in atr δ' δ :
-    auxtr_starts_in atr δ' → auxtr_starts_in (auxtr_extend atr δ) δ'.
-  Proof. induction atr; auto. Qed.
-
-  Lemma auxtr_extend_ends_in atr δ : auxtr_ends_in (auxtr_extend atr δ) δ.
-  Proof. done. Qed.
-
-End auxiliary_trace.
-
 Section system_trace.
-  Context `(AS : AuxState Λ).
+  Context `{AS : AuxState Λ}.
 
   Inductive valid_system_trace : execution_trace Λ → auxiliary_trace AS → Prop :=
   | valid_system_trace_singleton c δ :
-      valid_system_trace (singleton_exec c) (singleton_auxtr δ)
+      valid_system_trace (trace_singleton c) (trace_singleton δ)
   | valid_system_trace_step ex atr c c' δ δ' :
-      exec_ends_in ex c →
+      trace_ends_in ex c →
       step c c' →
-      auxtr_ends_in atr δ →
-      valid_state_evolution AS c.2 δ c'.2 δ' →
+      trace_ends_in atr δ →
+      valid_state_evolution ex atr c' δ' →
       valid_system_trace ex atr →
-      valid_system_trace (exec_extend ex c') (auxtr_extend atr δ').
+      valid_system_trace (trace_extend ex c') (trace_extend atr δ').
 
   Lemma valid_system_trace_valid_exec_trace ex atr :
     valid_system_trace ex atr → valid_exec ex.
   Proof. induction 1; econstructor; eauto. Qed.
 
   Lemma valid_system_trace_singletons c δ :
-    valid_system_trace (singleton_exec c) (singleton_auxtr δ).
+    valid_system_trace (trace_singleton c) (trace_singleton δ).
   Proof. constructor. Qed.
 
   Lemma valid_system_trace_extend ex atr c c' δ δ' :
     valid_system_trace ex atr →
-    exec_ends_in ex c →
+    trace_ends_in ex c →
     step c c' →
-    auxtr_ends_in atr δ →
-    valid_state_evolution AS c.2 δ c'.2 δ' →
-    valid_system_trace (exec_extend ex c') (auxtr_extend atr δ').
+    trace_ends_in atr δ →
+    valid_state_evolution ex atr c' δ' →
+    valid_system_trace (trace_extend ex c') (trace_extend atr δ').
   Proof.
     intros Heatr; revert c c' δ δ'.
     induction ex; econstructor; eauto.
   Qed.
 
   Lemma valid_system_trace_extend_inv ex atr c' δ' :
-    valid_system_trace (exec_extend ex c') (auxtr_extend atr δ') →
+    valid_system_trace (trace_extend ex c') (trace_extend atr δ') →
     ∃ c δ,
       valid_system_trace ex atr ∧
-      exec_ends_in ex c ∧
+      trace_ends_in ex c ∧
       step c c' ∧
-      auxtr_ends_in atr δ ∧
-      valid_state_evolution AS c.2 δ c'.2 δ'.
+      trace_ends_in atr δ ∧
+      valid_state_evolution ex atr c' δ'.
   Proof. inversion 1; eauto 10. Qed.
 
   Lemma valid_system_trace_ends_in ex atr :
-    valid_system_trace ex atr → ∃ c δ, exec_ends_in ex c ∧ auxtr_ends_in atr δ.
+    valid_system_trace ex atr → ∃ c δ, trace_ends_in ex c ∧ trace_ends_in atr δ.
   Proof.
     inversion 1;
-      eauto using exec_extend_ends_in, singleton_exec_ends_in,
-      auxtr_extend_ends_in, singleton_auxtr_ends_in.
+      eauto using trace_extend_ends_in, trace_singleton_ends_in,
+      trace_extend_ends_in, trace_singleton_ends_in.
   Qed.
 
 End system_trace.
@@ -246,13 +207,13 @@ Section simulation.
                 execution_trace Λ → auxiliary_trace AS → Prop) :
     execution_trace Λ → auxiliary_trace AS → Prop :=
     λ ex atr,
-    valid_system_trace AS ex atr ∧
+    valid_system_trace ex atr ∧
     φ ex atr ∧
     ∀ c c' δ,
-      exec_ends_in ex c →
-      auxtr_ends_in atr δ →
+      trace_ends_in ex c →
+      trace_ends_in atr δ →
       step c c' →
-      ∃ δ', continued_simulation (exec_extend ex c') (auxtr_extend atr δ').
+      ∃ δ', continued_simulation (trace_extend ex c') (trace_extend atr δ').
 
   Local Definition continued_simulation_pre_curried
         (φ : execution_trace Λ → auxiliary_trace AS → Prop) :
@@ -285,7 +246,7 @@ Section simulation.
   Qed.
 
   Lemma continued_simulation_valid_system_trace Φ ex tr:
-    continued_simulation Φ ex tr → valid_system_trace AS ex tr.
+    continued_simulation Φ ex tr → valid_system_trace ex tr.
   Proof.
     rewrite continued_simulation_unfold /continued_simulation_pre; intuition.
   Qed.
@@ -301,29 +262,29 @@ Section simulation.
              (ex : execution_trace Λ) (atr : auxiliary_trace AS)
              (c : cfg Λ) :
     continued_simulation φ ex atr →
-    valid_exec (exec_extend ex c) →
+    valid_exec (trace_extend ex c) →
     ∃ δ : aux_state AS,
-      continued_simulation φ (exec_extend ex c) (auxtr_extend atr δ).
+      continued_simulation φ (trace_extend ex c) (trace_extend atr δ).
   Proof.
     rewrite continued_simulation_unfold /continued_simulation_pre.
     intros (Hvst & HΦ & Hext) Hvex.
-    pose proof (valid_system_trace_ends_in _ _ _ Hvst) as (c1 & δ1 & Hc1 & Hδ1).
+    pose proof (valid_system_trace_ends_in _ _ Hvst) as (c1 & δ1 & Hc1 & Hδ1).
     apply valid_exec_exec_extend_inv in Hvex as [Hvex (c1' & Hc1' & Hstep)].
-    pose proof (exec_ends_in_inj _ _ _ Hc1 Hc1'); subst.
+    pose proof (trace_ends_in_inj _ _ _ Hc1 Hc1'); subst.
     eapply Hext; eauto.
   Qed.
 
   Lemma simulation_does_continue e σ δ φ :
-    continued_simulation φ (singleton_exec ([e], σ)) (singleton_auxtr δ) →
-    ∀ ex, exec_starts_in ex ([e], σ) → valid_exec ex →
+    continued_simulation φ (trace_singleton ([e], σ)) (trace_singleton δ) →
+    ∀ ex, trace_starts_in ex ([e], σ) → valid_exec ex →
           ∃ atr, continued_simulation φ ex atr.
   Proof.
     intros Hsm ex Hexstr Hex.
     induction Hex as [|? ? ? ? ? ? IHex].
-    - apply singleton_exec_starts_in_inv in Hexstr as ->.
-      exists (singleton_auxtr δ); eauto using valid_system_trace_singletons.
+    - apply trace_singleton_starts_in_inv in Hexstr as ->.
+      exists (trace_singleton δ); eauto using valid_system_trace_singletons.
     - destruct IHex as [atr Hsim].
-      { eapply exec_extend_starts_in_inv; eauto. }
+      { eapply trace_extend_starts_in_inv; eauto. }
       destruct (continued_simulation_next_aux_state_exists φ ex atr c');
         [done| |by eauto].
       econstructor; eauto.
